<?xml version="1.0" encoding="UTF-8"?>
<!DOCTYPE rdf:RDF [
	<!ENTITY dct "http://purl.org/dc/terms/">
	<!ENTITY fibo-fnd-aap-ppl "https://spec.edmcouncil.org/fibo/ontology/FND/AgentsAndPeople/People/">
	<!ENTITY fibo-fnd-arr-cls "https://spec.edmcouncil.org/fibo/ontology/FND/Arrangements/ClassificationSchemes/">
	<!ENTITY fibo-fnd-dt-fd "https://spec.edmcouncil.org/fibo/ontology/FND/DatesAndTimes/FinancialDates/">
	<!ENTITY fibo-fnd-pas-pas "https://spec.edmcouncil.org/fibo/ontology/FND/ProductsAndServices/ProductsAndServices/">
	<!ENTITY fibo-fnd-pty-pty "https://spec.edmcouncil.org/fibo/ontology/FND/Parties/Parties/">
	<!ENTITY fibo-fnd-pty-rl "https://spec.edmcouncil.org/fibo/ontology/FND/Parties/Roles/">
	<!ENTITY fibo-fnd-qt-qtu "https://spec.edmcouncil.org/fibo/ontology/FND/Quantities/QuantitiesAndUnits/">
	<!ENTITY fibo-fnd-rel-rel "https://spec.edmcouncil.org/fibo/ontology/FND/Relations/Relations/">
	<!ENTITY fibo-fnd-utl-alx "https://spec.edmcouncil.org/fibo/ontology/FND/Utilities/Analytics/">
	<!ENTITY fibo-fnd-utl-av "https://spec.edmcouncil.org/fibo/ontology/FND/Utilities/AnnotationVocabulary/">
	<!ENTITY lcc-cr "https://www.omg.org/spec/LCC/Countries/CountryRepresentation/">
	<!ENTITY lcc-lr "https://www.omg.org/spec/LCC/Languages/LanguageRepresentation/">
	<!ENTITY oe2020-pat-rec "https://tw.rpi.edu/ontology-engineering/oe2020/patient-guideline-recommender/">
	<!ENTITY owl "http://www.w3.org/2002/07/owl#">
	<!ENTITY rdf "http://www.w3.org/1999/02/22-rdf-syntax-ns#">
	<!ENTITY rdfs "http://www.w3.org/2000/01/rdf-schema#">
	<!ENTITY skos "http://www.w3.org/2004/02/skos/core#">
	<!ENTITY sm "http://www.omg.org/techprocess/ab/SpecificationMetadata/">
	<!ENTITY xsd "http://www.w3.org/2001/XMLSchema#">
]>
<rdf:RDF xml:base="https://tw.rpi.edu/ontology-engineering/oe2020/patient-guideline-recommender/"
	xmlns:dct="http://purl.org/dc/terms/"
	xmlns:fibo-fnd-aap-ppl="https://spec.edmcouncil.org/fibo/ontology/FND/AgentsAndPeople/People/"
	xmlns:fibo-fnd-arr-cls="https://spec.edmcouncil.org/fibo/ontology/FND/Arrangements/ClassificationSchemes/"
	xmlns:fibo-fnd-dt-fd="https://spec.edmcouncil.org/fibo/ontology/FND/DatesAndTimes/FinancialDates/"
	xmlns:fibo-fnd-pas-pas="https://spec.edmcouncil.org/fibo/ontology/FND/ProductsAndServices/ProductsAndServices/"
	xmlns:fibo-fnd-pty-pty="https://spec.edmcouncil.org/fibo/ontology/FND/Parties/Parties/"
	xmlns:fibo-fnd-pty-rl="https://spec.edmcouncil.org/fibo/ontology/FND/Parties/Roles/"
	xmlns:fibo-fnd-qt-qtu="https://spec.edmcouncil.org/fibo/ontology/FND/Quantities/QuantitiesAndUnits/"
	xmlns:fibo-fnd-rel-rel="https://spec.edmcouncil.org/fibo/ontology/FND/Relations/Relations/"
	xmlns:fibo-fnd-utl-alx="https://spec.edmcouncil.org/fibo/ontology/FND/Utilities/Analytics/"
	xmlns:fibo-fnd-utl-av="https://spec.edmcouncil.org/fibo/ontology/FND/Utilities/AnnotationVocabulary/"
	xmlns:lcc-cr="https://www.omg.org/spec/LCC/Countries/CountryRepresentation/"
	xmlns:lcc-lr="https://www.omg.org/spec/LCC/Languages/LanguageRepresentation/"
	xmlns:oe2020-pat-rec="https://tw.rpi.edu/ontology-engineering/oe2020/patient-guideline-recommender/"
	xmlns:owl="http://www.w3.org/2002/07/owl#"
	xmlns:rdf="http://www.w3.org/1999/02/22-rdf-syntax-ns#"
	xmlns:rdfs="http://www.w3.org/2000/01/rdf-schema#"
	xmlns:skos="http://www.w3.org/2004/02/skos/core#"
	xmlns:sm="http://www.omg.org/techprocess/ab/SpecificationMetadata/"
	xmlns:xsd="http://www.w3.org/2001/XMLSchema#">
	
	<owl:Ontology rdf:about="https://tw.rpi.edu/ontology-engineering/oe2020/patient-guideline-recommender/">
		<rdfs:label>Patient Guideline Recommender Ontology</rdfs:label>
		<dct:abstract>This ontology ...</dct:abstract>
		<sm:dependsOn rdf:datatype="&xsd;anyURI">https://spec.edmcouncil.org/fibo/ontology/FND/</sm:dependsOn>
		<sm:dependsOn rdf:datatype="&xsd;anyURI">https://www.omg.org/spec/LCC/</sm:dependsOn>
		<owl:imports rdf:resource="https://spec.edmcouncil.org/fibo/ontology/FND/AgentsAndPeople/People/"/>
		<owl:imports rdf:resource="https://spec.edmcouncil.org/fibo/ontology/FND/ClassificationSchemes/"/>
		<owl:imports rdf:resource="https://spec.edmcouncil.org/fibo/ontology/FND/DatesAndTimes/FinancialDates/"/>
		<owl:imports rdf:resource="https://spec.edmcouncil.org/fibo/ontology/FND/Parties/Parties/"/>
		<owl:imports rdf:resource="https://spec.edmcouncil.org/fibo/ontology/FND/Parties/Roles/"/>
		<owl:imports rdf:resource="https://spec.edmcouncil.org/fibo/ontology/FND/ProductsAndServices/ProductsAndServices/"/>
		<owl:imports rdf:resource="https://spec.edmcouncil.org/fibo/ontology/FND/Quantities/QuantitiesAndUnits/"/>
		<owl:imports rdf:resource="https://spec.edmcouncil.org/fibo/ontology/FND/Relations/Relations/"/>
		<owl:imports rdf:resource="https://spec.edmcouncil.org/fibo/ontology/FND/Utilities/Analytics/"/>
		<owl:imports rdf:resource="https://spec.edmcouncil.org/fibo/ontology/FND/Utilities/AnnotationVocabulary/"/>
		<owl:imports rdf:resource="https://www.omg.org/spec/LCC/Countries/CountryRepresentation/"/>
		<owl:imports rdf:resource="https://www.omg.org/spec/LCC/Languages/LanguageRepresentation/"/>
		<owl:versionIRI rdf:resource="https://tw.rpi.edu/ontology-engineering/oe2020/20201003/patient-guideline-recommender/"/>
		<skos:changeNote>The https://tw.rpi.edu/ontology-engineering/oe2020/20201003/patient-guideline-recommender.rdf version of this ontology is the seed version.</skos:changeNote>
	</owl:Ontology>
	
	<owl:Class rdf:about="&fibo-fnd-aap-ppl;Person">
		<rdfs:subClassOf>
			<owl:Restriction>
				<owl:onProperty rdf:resource="&oe2020-pat-rec;hasAge"/>
				<owl:someValuesFrom rdf:resource="&oe2020-pat-rec;PersonAge"/>
			</owl:Restriction>
		</rdfs:subClassOf>
		<rdfs:subClassOf>
			<owl:Restriction>
				<owl:onProperty rdf:resource="&oe2020-pat-rec;hasGenderIdentity"/>
				<owl:someValuesFrom rdf:resource="&oe2020-pat-rec;GenderIdentity"/>
			</owl:Restriction>
		</rdfs:subClassOf>
	</owl:Class>
	
	<owl:Class rdf:about="&oe2020-pat-rec;Age">
		<rdfs:subClassOf rdf:resource="&fibo-fnd-arr-cls;Classifier"/>
		<rdfs:subClassOf rdf:resource="&fibo-fnd-dt-fd;DatePeriod"/>
		<rdfs:subClassOf>
			<owl:Restriction>
				<owl:onProperty rdf:resource="&fibo-fnd-aap-ppl;hasStartDate"/>
				<owl:onClass rdf:resource="&fibo-fnd-dt-fd;ExplicitDate"/>
				<owl:qualifiedCardinality rdf:datatype="&xsd;nonNegativeInteger">1</owl:qualifiedCardinality>
			</owl:Restriction>
		</rdfs:subClassOf>
		<rdfs:label>age</rdfs:label>
		<skos:definition>period of time someone has been alive or something has existed</skos:definition>
		<fibo-fnd-utl-av:adaptedFrom rdf:datatype="&xsd;anyURI">https://dictionary.cambridge.org/dictionary/english/age</fibo-fnd-utl-av:adaptedFrom>
	</owl:Class>
	
	<owl:Class rdf:about="&oe2020-pat-rec;AgeGroup">
		<rdfs:subClassOf rdf:resource="&oe2020-pat-rec;Demographic"/>
		<rdfs:label>age group</rdfs:label>
		<skos:definition>demographic indicating a range of ages that a member of a population falls in at some point in time</skos:definition>
	</owl:Class>
	
	<owl:NamedIndividual rdf:about="&oe2020-pat-rec;Calorie">
		<rdf:type rdf:resource="&fibo-fnd-qt-qtu;DerivedUnit"/>
		<rdfs:label>Calorie</rdfs:label>
		<skos:definition>unit of energy widely used in nutrition</skos:definition>
		<fibo-fnd-utl-av:abbreviation>Cal</fibo-fnd-utl-av:abbreviation>
		<fibo-fnd-utl-av:abbreviation>kcal</fibo-fnd-utl-av:abbreviation>
		<fibo-fnd-utl-av:adaptedFrom rdf:datatype="&xsd;anyURI">https://en.wikipedia.org/wiki/Calorie</fibo-fnd-utl-av:adaptedFrom>
		<fibo-fnd-utl-av:explanatoryNote>The large calorie, food calorie, or kilocalorie (Cal, Calorie or kcal) is the amount of heat needed to cause the same increase in one kilogram of water (i.e., 4184 J). Thus, 1 kilocalorie (kcal) = 1000 calories (cal). By convention in food science, the large calorie is commonly called Calorie (with a capital C by some authors to distinguish from the smaller unit). In most countries, labels of industrialized food products are required to indicate the nutritional energy value in (kilo or large) calories per serving or per weight.</fibo-fnd-utl-av:explanatoryNote>
	</owl:NamedIndividual>
	
	<owl:Class rdf:about="&oe2020-pat-rec;DateOfBirth">
		<rdfs:subClassOf rdf:resource="&fibo-fnd-dt-fd;ExplicitDate"/>
		<rdfs:label>date of birth</rdfs:label>
		<skos:definition>explicit date on which an individual was born</skos:definition>
		<fibo-fnd-utl-av:synonym>birth date</fibo-fnd-utl-av:synonym>
		<fibo-fnd-utl-av:synonym>birthday</fibo-fnd-utl-av:synonym>
	</owl:Class>
	
	<owl:Class rdf:about="&oe2020-pat-rec;DeclinedToState">
		<rdfs:subClassOf rdf:resource="&oe2020-pat-rec;GenderIdentity"/>
		<rdfs:label>declined to state</rdfs:label>
		<skos:definition>gender identity indicating that the individual chose not to provide information as of some date</skos:definition>
	</owl:Class>
	
	<owl:Class rdf:about="&oe2020-pat-rec;Demographic">
		<rdfs:subClassOf rdf:resource="&fibo-fnd-arr-cls;Classifier"/>
		<rdfs:subClassOf>
			<owl:Restriction>
				<owl:onProperty rdf:resource="&lcc-cr;classifies"/>
				<owl:someValuesFrom rdf:resource="&fibo-fnd-aap-ppl;Person"/>
			</owl:Restriction>
		</rdfs:subClassOf>
		<rdfs:label>demographic</rdfs:label>
		<skos:definition>statistical characteristic of a human population (such as age or income)</skos:definition>
		<fibo-fnd-utl-av:adaptedFrom>A. B. Olokoba, O. A. Obateru, and L. B. Olokoba, &apos;Type 2 diabetes mellitus: a review of current trends,&apos; Oman medical journal, Jul-2012. [Online]. Available: https://www.ncbi.nlm.nih.gov/pmc/articles/PMC3464757/?fbclid=IwAR08ScAD3TqjSQm569uKaPu1sbcpCxzKI0gHXeuY9WsSgFUDMlBes5Xxhdg. [Accessed: 23-Sep-2020].</fibo-fnd-utl-av:adaptedFrom>
	</owl:Class>
	
	<owl:Class rdf:about="&oe2020-pat-rec;Diet">
		<rdfs:subClassOf rdf:resource="&lcc-lr;Collection"/>
		<rdfs:subClassOf>
			<owl:Restriction>
				<owl:onProperty rdf:resource="&fibo-fnd-rel-rel;comprises"/>
				<owl:someValuesFrom rdf:resource="&oe2020-pat-rec;Food"/>
			</owl:Restriction>
		</rdfs:subClassOf>
		<rdfs:label>diet</rdfs:label>
		<skos:definition>prescribed course of eating and drinking in which the amount and kind of food, as well as the times at which it is to be taken, are regulated for therapeutic purposes or selected with reference to a particular state of health</skos:definition>
		<fibo-fnd-utl-av:adaptedFrom>S. Chong, D. Ding, R. Byun, E. Comino, A. Bauman, and B. Jalaludin, &apos;Lifestyle Changes After a Diagnosis of Type 2 Diabetes,&apos; Diabetes spectrum : a publication of the American Diabetes Association, Feb-2017. [Online]. Available: https://www.ncbi.nlm.nih.gov/pmc/articles/PMC5309903/?fbclid=IwAR2dY5OKOjSBRXRGfKAQ4NQosTKp534nixdd8ac6KW55BT3SmFSTitGHbbY. [Accessed: 23-Sep-2020].</fibo-fnd-utl-av:adaptedFrom>
	</owl:Class>
	
	<owl:Class rdf:about="&oe2020-pat-rec;Female">
		<rdfs:subClassOf rdf:resource="&oe2020-pat-rec;GenderIdentity"/>
		<rdfs:label>female</rdfs:label>
		<skos:definition>gender identity indicating that the individual self-identifies as being a woman</skos:definition>
	</owl:Class>
	
	<owl:NamedIndividual rdf:about="&oe2020-pat-rec;FemaleGroup">
		<rdf:type rdf:resource="&oe2020-pat-rec;GenderIdentityGroup"/>
		<rdfs:label>female group</rdfs:label>
		<skos:definition>gender identity group including individuals that self-identify as female</skos:definition>
	</owl:NamedIndividual>
	
	<owl:Class rdf:about="&oe2020-pat-rec;Food">
		<rdfs:subClassOf rdf:resource="&fibo-fnd-pas-pas;Product"/>
		<rdfs:label>food</rdfs:label>
		<skos:definition>material consisting essentially of protein, carbohydrate, and fat used in the body of an organism to sustain growth, repair, and vital processes and to furnish energy</skos:definition>
		<fibo-fnd-utl-av:adaptedFrom rdf:datatype="&xsd;anyURI">https://www.merriam-webster.com/dictionary/food</fibo-fnd-utl-av:adaptedFrom>
	</owl:Class>
	
	<owl:Class rdf:about="&oe2020-pat-rec;GenderIdentity">
		<rdfs:subClassOf rdf:resource="&fibo-fnd-arr-cls;Classifier"/>
		<rdfs:subClassOf>
			<owl:Restriction>
				<owl:onProperty rdf:resource="&fibo-fnd-dt-fd;hasAsOfDate"/>
				<owl:onClass rdf:resource="&fibo-fnd-dt-fd;ExplicitDate"/>
				<owl:qualifiedCardinality rdf:datatype="&xsd;nonNegativeInteger">1</owl:qualifiedCardinality>
			</owl:Restriction>
		</rdfs:subClassOf>
		<rdfs:label>gender identity</rdfs:label>
		<skos:definition>classifier indicating one&apos;s personal experience of one&apos;s own gender</skos:definition>
	</owl:Class>
	
	<owl:Class rdf:about="&oe2020-pat-rec;GenderIdentityGroup">
		<rdfs:subClassOf rdf:resource="&oe2020-pat-rec;Demographic"/>
		<rdfs:label>gender identity group</rdfs:label>
		<skos:definition>demographic indicating a qualitative value for gender identity that a member of a population identifies with at some point in time</skos:definition>
	</owl:Class>
	
	<owl:Class rdf:about="&oe2020-pat-rec;Male">
		<rdfs:subClassOf rdf:resource="&oe2020-pat-rec;GenderIdentity"/>
		<rdfs:label>male</rdfs:label>
		<skos:definition>gender identity indicating that the individual self-identifies as being a man</skos:definition>
	</owl:Class>
	
	<owl:NamedIndividual rdf:about="&oe2020-pat-rec;MaleGroup">
		<rdf:type rdf:resource="&oe2020-pat-rec;GenderIdentityGroup"/>
		<rdfs:label>male group</rdfs:label>
		<skos:definition>gender identity group including individuals that self-identify as male</skos:definition>
	</owl:NamedIndividual>
	
	<owl:Class rdf:about="&oe2020-pat-rec;NonBinary">
		<rdfs:subClassOf rdf:resource="&oe2020-pat-rec;GenderIdentity"/>
		<rdfs:label>non-binary</rdfs:label>
		<skos:definition>gender identity indicating that the individual self-identifies as not being exclusively masculine or feminine, i.e., as being outside of the gender binary</skos:definition>
	</owl:Class>
	
	<owl:NamedIndividual rdf:about="&oe2020-pat-rec;NonBinaryGroup">
		<rdf:type rdf:resource="&oe2020-pat-rec;GenderIdentityGroup"/>
		<rdfs:label>non-binary group</rdfs:label>
		<skos:definition>gender identity group including individuals that self-identify as not being exclusively masculine or feminine, i.e., as being outside of the gender binary</skos:definition>
	</owl:NamedIndividual>
	
	<owl:NamedIndividual rdf:about="&oe2020-pat-rec;None">
		<rdf:type rdf:resource="&oe2020-pat-rec;GenderIdentityGroup"/>
		<rdfs:label>none</rdfs:label>
		<skos:definition>gender identity group including individuals that do not self-identify as belonging to any defined group</skos:definition>
	</owl:NamedIndividual>
	
	<owl:Class rdf:about="&oe2020-pat-rec;Patient">
		<rdfs:subClassOf rdf:resource="&fibo-fnd-pty-pty;PartyInRole"/>
		<rdfs:subClassOf>
			<owl:Restriction>
				<owl:onProperty rdf:resource="&fibo-fnd-rel-rel;hasIdentity"/>
				<owl:onClass rdf:resource="&fibo-fnd-aap-ppl;Person"/>
				<owl:qualifiedCardinality rdf:datatype="&xsd;nonNegativeInteger">1</owl:qualifiedCardinality>
			</owl:Restriction>
		</rdfs:subClassOf>
		<rdfs:label>patient</rdfs:label>
		<skos:definition>person who receives medical attention, care, or treatment, or who is registered with medical professional or institution with the purpose to receive medical care when necessary</skos:definition>
		<skos:scopeNote>Patients will be limited to those who have type 2 diabetes.</skos:scopeNote>
		<fibo-fnd-utl-av:adaptedFrom>S. Chong, D. Ding, R. Byun, E. Comino, A. Bauman, and B. Jalaludin, &apos;Lifestyle Changes After a Diagnosis of Type 2 Diabetes,&apos; Diabetes spectrum : a publication of the American Diabetes Association, Feb-2017. [Online]. Available: https://www.ncbi.nlm.nih.gov/pmc/articles/PMC5309903/?fbclid=IwAR2dY5OKOjSBRXRGfKAQ4NQosTKp534nixdd8ac6KW55BT3SmFSTitGHbbY. [Accessed: 23-Sep-2020].</fibo-fnd-utl-av:adaptedFrom>
	</owl:Class>
	
	<owl:Class rdf:about="&oe2020-pat-rec;PersonAge">
		<rdfs:subClassOf rdf:resource="&oe2020-pat-rec;Age"/>
		<rdfs:subClassOf>
			<owl:Restriction>
				<owl:onProperty rdf:resource="&fibo-fnd-dt-fd;hasAsOfDate"/>
				<owl:onClass rdf:resource="&fibo-fnd-dt-fd;ExplicitDate"/>
				<owl:qualifiedCardinality rdf:datatype="&xsd;nonNegativeInteger">1</owl:qualifiedCardinality>
			</owl:Restriction>
		</rdfs:subClassOf>
		<rdfs:subClassOf>
			<owl:Restriction>
				<owl:onProperty rdf:resource="&oe2020-pat-rec;isCalculatedFromBirth"/>
				<owl:onClass rdf:resource="&oe2020-pat-rec;DateOfBirth"/>
				<owl:qualifiedCardinality rdf:datatype="&xsd;nonNegativeInteger">1</owl:qualifiedCardinality>
			</owl:Restriction>
		</rdfs:subClassOf>
		<rdfs:label>person age</rdfs:label>
		<skos:definition>period of time a person has been alive</skos:definition>
		<fibo-fnd-utl-av:adaptedFrom rdf:datatype="&xsd;anyURI">https://dictionary.cambridge.org/dictionary/english/age</fibo-fnd-utl-av:adaptedFrom>
	</owl:Class>
	
	<owl:Class rdf:about="&oe2020-pat-rec;Transgender">
		<rdfs:subClassOf rdf:resource="&oe2020-pat-rec;GenderIdentity"/>
		<rdfs:label>transgender</rdfs:label>
		<skos:definition>gender identity indicating that the individual self-identifies as having a gender identity or gender expression that differs with their assigned sex at birth</skos:definition>
	</owl:Class>
	
	<owl:NamedIndividual rdf:about="&oe2020-pat-rec;TransgenderGroup">
		<rdf:type rdf:resource="&oe2020-pat-rec;GenderIdentityGroup"/>
		<rdfs:label>transgender group</rdfs:label>
		<skos:definition>gender identity including individuals that self-identify as having a gender identity or gender expression that differs with their assigned sex at birth</skos:definition>
	</owl:NamedIndividual>
	
	<owl:ObjectProperty rdf:about="&oe2020-pat-rec;hasAge">
		<rdfs:subPropertyOf rdf:resource="&fibo-fnd-rel-rel;isCharacterizedBy"/>
		<rdfs:label>has age</rdfs:label>
		<rdfs:range rdf:resource="&oe2020-pat-rec;Age"/>
		<skos:definition>indicates the length of time someone has been alive or something has existed</skos:definition>
	</owl:ObjectProperty>
	
	<owl:ObjectProperty rdf:about="&oe2020-pat-rec;hasGenderIdentity">
		<rdfs:subPropertyOf rdf:resource="&fibo-fnd-rel-rel;isCharacterizedBy"/>
		<rdfs:label>has gender identity</rdfs:label>
		<rdfs:range rdf:resource="&oe2020-pat-rec;GenderIdentity"/>
		<skos:definition>indicates the gender as reported by an individual</skos:definition>
	</owl:ObjectProperty>
	
	<owl:ObjectProperty rdf:about="&oe2020-pat-rec;isCalculatedFromBirth">
		<rdfs:subPropertyOf rdf:resource="&fibo-fnd-aap-ppl;hasStartDate"/>
		<rdfs:label>is calculated from birth</rdfs:label>
		<rdfs:range rdf:resource="&oe2020-pat-rec;DateOfBirth"/>
		<skos:definition>indicates the date from which age is calculated</skos:definition>
		<fibo-fnd-utl-av:adaptedFrom rdf:datatype="&xsd;anyURI">https://dictionary.cambridge.org/dictionary/english/age</fibo-fnd-utl-av:adaptedFrom>
	</owl:ObjectProperty>

</rdf:RDF>